Adjust tvsubst operations to use explicit carrier set

operations/TVSubst.thy
@@ -67,6 +67,72 @@ definition asVVr12 :: "('var::{var_T1_pre, var_T2_pre}, 'tyvar::{var_T1_pre, var
 definition asVVr21 :: "('var::{var_T1_pre, var_T2_pre}, 'tyvar::{var_T1_pre, var_T2_pre}, 'a::{var_T1_pre, var_T2_pre}, 'b) T2 \<Rightarrow> 'var" where
   "asVVr21 x \<equiv> (if isVVr21 x then SOME a. x = VVr21 a else undefined)"
 
+type_synonym ('var, 'tyvar, 'a, 'b) SSfun11 = "'var \<Rightarrow> ('var, 'tyvar, 'a, 'b) T1"
+type_synonym ('var, 'tyvar, 'a, 'b) SSfun12 = "'tyvar \<Rightarrow> ('var, 'tyvar, 'a, 'b) T1"
+type_synonym ('var, 'tyvar, 'a, 'b) SSfun21 = "'var \<Rightarrow> ('var, 'tyvar, 'a, 'b) T2"
+
+definition compSS11 :: "('var \<Rightarrow> 'var) \<Rightarrow> ('tyvar \<Rightarrow> 'tyvar) \<Rightarrow> ('var, 'tyvar, 'a, 'b) SSfun11 \<Rightarrow> ('var::{var_T1_pre, var_T2_pre}, 'tyvar::{var_T1_pre, var_T2_pre}, 'a::{var_T1_pre, var_T2_pre}, 'b) SSfun11" where
+  "compSS11 f1 f2 h \<equiv> rrename_T1 f1 f2 \<circ> h \<circ> inv f1"
+definition compSS12 :: "('var \<Rightarrow> 'var) \<Rightarrow> ('tyvar \<Rightarrow> 'tyvar) \<Rightarrow> ('var, 'tyvar, 'a, 'b) SSfun12 \<Rightarrow> ('var::{var_T1_pre, var_T2_pre}, 'tyvar::{var_T1_pre, var_T2_pre}, 'a::{var_T1_pre, var_T2_pre}, 'b) SSfun12" where
+  "compSS12 f1 f2 h \<equiv> rrename_T1 f1 f2 \<circ> h \<circ> inv f2"
+definition compSS21 :: "('var \<Rightarrow> 'var) \<Rightarrow> ('tyvar \<Rightarrow> 'tyvar) \<Rightarrow> ('var, 'tyvar, 'a, 'b) SSfun21 \<Rightarrow> ('var::{var_T1_pre, var_T2_pre}, 'tyvar::{var_T1_pre, var_T2_pre}, 'a::{var_T1_pre, var_T2_pre}, 'b) SSfun21" where
+  "compSS21 f1 f2 h \<equiv> rrename_T2 f1 f2 \<circ> h \<circ> inv f1"
+lemmas compSS_defs = compSS11_def compSS12_def compSS21_def
+
+type_synonym ('var, 'tyvar, 'a, 'b) P = "('var, 'tyvar, 'a, 'b) SSfun11 \<times> ('var, 'tyvar, 'a, 'b) SSfun12 \<times> ('var, 'tyvar, 'a, 'b) SSfun21"
+type_synonym ('var, 'tyvar, 'a, 'b) U1 = "('var, 'tyvar, 'a, 'b) T1"
+type_synonym ('var, 'tyvar, 'a, 'b) U2 = "('var, 'tyvar, 'a, 'b) T2"
+
+definition U1ctor :: "('var::{var_T1_pre, var_T2_pre}, 'tyvar::{var_T1_pre, var_T2_pre}, 'a::{var_T1_pre, var_T2_pre}, 'b, 'var, 'tyvar, ('var, 'tyvar, 'a, 'b) T1 \<times> (('var, 'tyvar, 'a, 'b) P \<Rightarrow> ('var, 'tyvar, 'a, 'b) U1), ('var, 'tyvar, 'a, 'b) T1 \<times> (('var, 'tyvar, 'a, 'b) P \<Rightarrow> ('var, 'tyvar, 'a, 'b) U1),
+  ('var, 'tyvar, 'a, 'b) T2 \<times> (('var, 'tyvar, 'a, 'b) P \<Rightarrow> ('var, 'tyvar, 'a, 'b) U2), ('var, 'tyvar, 'a, 'b) T2 \<times> (('var, 'tyvar, 'a, 'b) P \<Rightarrow> ('var, 'tyvar, 'a, 'b) U2)) T1_pre \<Rightarrow> ('var, 'tyvar, 'a, 'b) P \<Rightarrow> ('var, 'tyvar, 'a, 'b) U1" where
+  "U1ctor y p \<equiv> case p of (f1, f2, f3) \<Rightarrow> if isVVr11 (T1_ctor (map_T1_pre id id id id id id fst fst fst fst y)) then
+    f1 (asVVr11 (T1_ctor (map_T1_pre id id id id id id fst fst fst fst y))) else (
+  if isVVr12 (T1_ctor (map_T1_pre id id id id id id fst fst fst fst y)) then
+    f2 (asVVr12 (T1_ctor (map_T1_pre id id id id id id fst fst fst fst y))) else (
+  T1_ctor (map_T1_pre id id id id id id ((\<lambda>R. R (f1, f2, f3)) \<circ> snd) ((\<lambda>R. R (f1, f2, f3)) \<circ> snd) ((\<lambda>R. R (f1, f2, f3)) \<circ> snd) ((\<lambda>R. R (f1, f2, f3)) \<circ> snd) y)
+))"
+definition U2ctor :: "('var::{var_T1_pre, var_T2_pre}, 'tyvar::{var_T1_pre, var_T2_pre}, 'a::{var_T1_pre, var_T2_pre}, 'b, 'var, 'tyvar, ('var, 'tyvar, 'a, 'b) T1 \<times> (('var, 'tyvar, 'a, 'b) P \<Rightarrow> ('var, 'tyvar, 'a, 'b) U1), ('var, 'tyvar, 'a, 'b) T1 \<times> (('var, 'tyvar, 'a, 'b) P \<Rightarrow> ('var, 'tyvar, 'a, 'b) U1),
+  ('var, 'tyvar, 'a, 'b) T2 \<times> (('var, 'tyvar, 'a, 'b) P \<Rightarrow> ('var, 'tyvar, 'a, 'b) U2), ('var, 'tyvar, 'a, 'b) T2 \<times> (('var, 'tyvar, 'a, 'b) P \<Rightarrow> ('var, 'tyvar, 'a, 'b) U2)) T2_pre \<Rightarrow> ('var, 'tyvar, 'a, 'b) P \<Rightarrow> ('var, 'tyvar, 'a, 'b) U2" where
+  "U2ctor y p \<equiv> case p of (f1, f2, f3) \<Rightarrow> if isVVr21 (T2_ctor (map_T2_pre id id id id id id fst fst fst fst y)) then
+    f3 (asVVr21 (T2_ctor (map_T2_pre id id id id id id fst fst fst fst y))) else (
+  T2_ctor (map_T2_pre id id id id id id ((\<lambda>R. R (f1, f2, f3)) \<circ> snd) ((\<lambda>R. R (f1, f2, f3)) \<circ> snd) ((\<lambda>R. R (f1, f2, f3)) \<circ> snd) ((\<lambda>R. R (f1, f2, f3)) \<circ> snd) y)
+)"
+
+definition PFVars_1 :: "('var::{var_T1_pre,var_T2_pre}, 'tyvar::{var_T1_pre,var_T2_pre}, 'a::{var_T1_pre,var_T2_pre}, 'b) P \<Rightarrow> 'var set" where
+  "PFVars_1 p \<equiv> case p of (f1, f2, f3) \<Rightarrow> IImsupp11_1 f1 \<union> IImsupp12_1 f2 \<union> IImsupp21_1 f3"
+definition PFVars_2 :: "('var::{var_T1_pre,var_T2_pre}, 'tyvar::{var_T1_pre,var_T2_pre}, 'a::{var_T1_pre,var_T2_pre}, 'b) P \<Rightarrow> 'tyvar set" where
+  "PFVars_2 p \<equiv> case p of (f1, f2, f3) \<Rightarrow> IImsupp11_2 f1 \<union> IImsupp12_2 f2 \<union> IImsupp21_2 f3"
+
+definition Pmap :: "('var \<Rightarrow> 'var) \<Rightarrow> ('tyvar \<Rightarrow> 'tyvar) \<Rightarrow> ('var::{var_T1_pre,var_T2_pre}, 'tyvar::{var_T1_pre,var_T2_pre}, 'a::{var_T1_pre,var_T2_pre}, 'b) P \<Rightarrow> ('var, 'tyvar, 'a, 'b) P" where
+  "Pmap g1 g2 p \<equiv> case p of (f1, f2, f3) \<Rightarrow> (compSS11 g1 g2 f1, compSS12 g1 g2 f2, compSS21 g1 g2 f3)"
+
+definition avoiding_set1 :: "'var::{var_T1_pre,var_T2_pre} set" where "avoiding_set1 \<equiv> {}"
+definition avoiding_set2 :: "'tyvar::{var_T1_pre,var_T2_pre} set" where "avoiding_set2 \<equiv> {}"
+
+abbreviation "U1FVars_1 \<equiv> \<lambda>(_::('var, 'tyvar, 'a, 'b) T1) (x::('var::{var_T1_pre,var_T2_pre}, 'tyvar::{var_T1_pre,var_T2_pre}, 'a::{var_T1_pre,var_T2_pre}, 'b) T1). FFVars_T11 x"
+abbreviation "U1FVars_2 \<equiv> \<lambda>(_::('var, 'tyvar, 'a, 'b) T1) (x::('var::{var_T1_pre,var_T2_pre}, 'tyvar::{var_T1_pre,var_T2_pre}, 'a::{var_T1_pre,var_T2_pre}, 'b) T1). FFVars_T12 x"
+abbreviation "U2FVars_1 \<equiv> \<lambda>(_::('var, 'tyvar, 'a, 'b) T2) (x::('var::{var_T1_pre,var_T2_pre}, 'tyvar::{var_T1_pre,var_T2_pre}, 'a::{var_T1_pre,var_T2_pre}, 'b) T2). FFVars_T21 x"
+abbreviation "U2FVars_2 \<equiv> \<lambda>(_::('var, 'tyvar, 'a, 'b) T2) (x::('var::{var_T1_pre,var_T2_pre}, 'tyvar::{var_T1_pre,var_T2_pre}, 'a::{var_T1_pre,var_T2_pre}, 'b) T2). FFVars_T22 x"
+
+abbreviation "U1map \<equiv> \<lambda>f1 f2 (_::('var, 'tyvar, 'a, 'b) T1) (x::('var::{var_T1_pre,var_T2_pre}, 'tyvar::{var_T1_pre,var_T2_pre}, 'a::{var_T1_pre,var_T2_pre}, 'b) T1). rrename_T1 f1 f2 x"
+abbreviation "U2map \<equiv> \<lambda>f1 f2 (_::('var, 'tyvar, 'a, 'b) T2) (x::('var::{var_T1_pre,var_T2_pre}, 'tyvar::{var_T1_pre,var_T2_pre}, 'a::{var_T1_pre,var_T2_pre}, 'b) T2). rrename_T2 f1 f2 x"
+
+definition valid_P :: "('var::{var_T1_pre,var_T2_pre}, 'tyvar::{var_T1_pre,var_T2_pre}, 'a::{var_T1_pre,var_T2_pre}, 'b) P \<Rightarrow> bool" where
+  "valid_P p \<equiv> case p of (f1, f2, f3) \<Rightarrow>
+  |SSupp11 f1| <o cmin |UNIV::'var set| |UNIV::'tyvar set|
+  \<and> |SSupp12 f2| <o cmin |UNIV::'var set| |UNIV::'tyvar set|
+  \<and> |SSupp21 f3| <o cmin |UNIV::'var set| |UNIV::'tyvar set|"
+
+(**********************************************************************)
+(*                               PROOFS                               *)
+(**********************************************************************)
+
+lemmas Cinfinite_UNIV = conjI[OF T1_pre.UNIV_cinfinite card_of_Card_order]
+lemmas Cinfinite_card = cmin_Cinfinite[OF Cinfinite_UNIV Cinfinite_UNIV]
+lemmas regularCard_card = cmin_regularCard[OF T1_pre.var_regular T1_pre.var_regular Cinfinite_UNIV Cinfinite_UNIV]
+lemmas Un_bound = regularCard_Un[OF conjunct2[OF Cinfinite_card] conjunct1[OF Cinfinite_card] regularCard_card]
+lemmas UNION_bound = regularCard_UNION[OF conjunct2[OF Cinfinite_card] conjunct1[OF Cinfinite_card] regularCard_card]
+
 lemma Supp_VVr_empty:
   "SSupp11 VVr11 = {}"
   "SSupp12 VVr12 = {}"
@@ -98,82 +164,6 @@ lemma SSupp_VVr_bound:
     apply (unfold Supp_VVr_empty)
     apply (rule emp_bound)+
   done
-
-typedef (overloaded) ('var, 'tyvar, 'a, 'b) SSfun11 = "{ f. |SSupp11 (f::_ \<Rightarrow> ('var::{var_T1_pre, var_T2_pre}, 'tyvar::{var_T1_pre, var_T2_pre}, 'a::{var_T1_pre, var_T2_pre}, 'b) T1)| <o cmin |UNIV::'var set| |UNIV::'tyvar set| }"
-  apply (rule exI)
-  apply (rule iffD2[OF mem_Collect_eq])
-  apply (rule cmin_greater)
-     apply (rule card_of_Card_order SSupp_VVr_bound)+
-  done
-
-typedef (overloaded) ('var, 'tyvar, 'a, 'b) SSfun12 = "{ f. |SSupp12 (f::_ \<Rightarrow> ('var::{var_T1_pre, var_T2_pre}, 'tyvar::{var_T1_pre, var_T2_pre}, 'a::{var_T1_pre, var_T2_pre}, 'b) T1)| <o  cmin |UNIV::'var set| |UNIV::'tyvar set| }"
-  apply (rule exI)
-  apply (rule iffD2[OF mem_Collect_eq])
-  apply (rule cmin_greater)
-     apply (rule card_of_Card_order SSupp_VVr_bound)+
-  done
-
-typedef (overloaded) ('var, 'tyvar, 'a, 'b) SSfun21 = "{ f. |SSupp21 (f::_ \<Rightarrow> ('var::{var_T1_pre, var_T2_pre}, 'tyvar::{var_T1_pre, var_T2_pre}, 'a::{var_T1_pre, var_T2_pre}, 'b) T2)| <o  cmin |UNIV::'var set| |UNIV::'tyvar set| }"
-  apply (rule exI)
-  apply (rule iffD2[OF mem_Collect_eq])
-  apply (rule cmin_greater)
-     apply (rule card_of_Card_order SSupp_VVr_bound)+
-  done
-
-definition compSS11 :: "('var \<Rightarrow> 'var) \<Rightarrow> ('tyvar \<Rightarrow> 'tyvar) \<Rightarrow> ('var, 'tyvar, 'a, 'b) SSfun11 \<Rightarrow> ('var::{var_T1_pre, var_T2_pre}, 'tyvar::{var_T1_pre, var_T2_pre}, 'a::{var_T1_pre, var_T2_pre}, 'b) SSfun11" where
-  "compSS11 f1 f2 p \<equiv> Abs_SSfun11 (rrename_T1 f1 f2 \<circ> Rep_SSfun11 p \<circ> inv f1)"
-definition compSS12 :: "('var \<Rightarrow> 'var) \<Rightarrow> ('tyvar \<Rightarrow> 'tyvar) \<Rightarrow> ('var, 'tyvar, 'a, 'b) SSfun12 \<Rightarrow> ('var::{var_T1_pre, var_T2_pre}, 'tyvar::{var_T1_pre, var_T2_pre}, 'a::{var_T1_pre, var_T2_pre}, 'b) SSfun12" where
-  "compSS12 f1 f2 p \<equiv> Abs_SSfun12 (rrename_T1 f1 f2 \<circ> Rep_SSfun12 p \<circ> inv f2)"
-definition compSS21 :: "('var \<Rightarrow> 'var) \<Rightarrow> ('tyvar \<Rightarrow> 'tyvar) \<Rightarrow> ('var, 'tyvar, 'a, 'b) SSfun21 \<Rightarrow> ('var::{var_T1_pre, var_T2_pre}, 'tyvar::{var_T1_pre, var_T2_pre}, 'a::{var_T1_pre, var_T2_pre}, 'b) SSfun21" where
-  "compSS21 f1 f2 p \<equiv> Abs_SSfun21 (rrename_T2 f1 f2 \<circ> Rep_SSfun21 p \<circ> inv f1)"
-
-type_synonym ('var, 'tyvar, 'a, 'b) P = "('var, 'tyvar, 'a, 'b) SSfun11 \<times> ('var, 'tyvar, 'a, 'b) SSfun12 \<times> ('var, 'tyvar, 'a, 'b) SSfun21"
-type_synonym ('var, 'tyvar, 'a, 'b) U1 = "('var, 'tyvar, 'a, 'b) T1"
-type_synonym ('var, 'tyvar, 'a, 'b) U2 = "('var, 'tyvar, 'a, 'b) T2"
-
-definition U1ctor :: "('var::{var_T1_pre, var_T2_pre}, 'tyvar::{var_T1_pre, var_T2_pre}, 'a::{var_T1_pre, var_T2_pre}, 'b, 'var, 'tyvar, ('var, 'tyvar, 'a, 'b) T1 \<times> (('var, 'tyvar, 'a, 'b) P \<Rightarrow> ('var, 'tyvar, 'a, 'b) U1), ('var, 'tyvar, 'a, 'b) T1 \<times> (('var, 'tyvar, 'a, 'b) P \<Rightarrow> ('var, 'tyvar, 'a, 'b) U1),
-  ('var, 'tyvar, 'a, 'b) T2 \<times> (('var, 'tyvar, 'a, 'b) P \<Rightarrow> ('var, 'tyvar, 'a, 'b) U2), ('var, 'tyvar, 'a, 'b) T2 \<times> (('var, 'tyvar, 'a, 'b) P \<Rightarrow> ('var, 'tyvar, 'a, 'b) U2)) T1_pre \<Rightarrow> ('var, 'tyvar, 'a, 'b) P \<Rightarrow> ('var, 'tyvar, 'a, 'b) U1" where
-  "U1ctor y p \<equiv> case p of (f1, f2, f3) \<Rightarrow> if isVVr11 (T1_ctor (map_T1_pre id id id id id id fst fst fst fst y)) then
-    Rep_SSfun11 f1 (asVVr11 (T1_ctor (map_T1_pre id id id id id id fst fst fst fst y))) else (
-  if isVVr12 (T1_ctor (map_T1_pre id id id id id id fst fst fst fst y)) then
-    Rep_SSfun12 f2 (asVVr12 (T1_ctor (map_T1_pre id id id id id id fst fst fst fst y))) else (
-  T1_ctor (map_T1_pre id id id id id id ((\<lambda>R. R (f1, f2, f3)) \<circ> snd) ((\<lambda>R. R (f1, f2, f3)) \<circ> snd) ((\<lambda>R. R (f1, f2, f3)) \<circ> snd) ((\<lambda>R. R (f1, f2, f3)) \<circ> snd) y)
-))"
-definition U2ctor :: "('var::{var_T1_pre, var_T2_pre}, 'tyvar::{var_T1_pre, var_T2_pre}, 'a::{var_T1_pre, var_T2_pre}, 'b, 'var, 'tyvar, ('var, 'tyvar, 'a, 'b) T1 \<times> (('var, 'tyvar, 'a, 'b) P \<Rightarrow> ('var, 'tyvar, 'a, 'b) U1), ('var, 'tyvar, 'a, 'b) T1 \<times> (('var, 'tyvar, 'a, 'b) P \<Rightarrow> ('var, 'tyvar, 'a, 'b) U1),
-  ('var, 'tyvar, 'a, 'b) T2 \<times> (('var, 'tyvar, 'a, 'b) P \<Rightarrow> ('var, 'tyvar, 'a, 'b) U2), ('var, 'tyvar, 'a, 'b) T2 \<times> (('var, 'tyvar, 'a, 'b) P \<Rightarrow> ('var, 'tyvar, 'a, 'b) U2)) T2_pre \<Rightarrow> ('var, 'tyvar, 'a, 'b) P \<Rightarrow> ('var, 'tyvar, 'a, 'b) U2" where
-  "U2ctor y p \<equiv> case p of (f1, f2, f3) \<Rightarrow> if isVVr21 (T2_ctor (map_T2_pre id id id id id id fst fst fst fst y)) then
-    Rep_SSfun21 f3 (asVVr21 (T2_ctor (map_T2_pre id id id id id id fst fst fst fst y))) else (
-  T2_ctor (map_T2_pre id id id id id id ((\<lambda>R. R (f1, f2, f3)) \<circ> snd) ((\<lambda>R. R (f1, f2, f3)) \<circ> snd) ((\<lambda>R. R (f1, f2, f3)) \<circ> snd) ((\<lambda>R. R (f1, f2, f3)) \<circ> snd) y)
-)"
-
-definition PFVars_1 :: "('var::{var_T1_pre,var_T2_pre}, 'tyvar::{var_T1_pre,var_T2_pre}, 'a::{var_T1_pre,var_T2_pre}, 'b) P \<Rightarrow> 'var set" where
-  "PFVars_1 p \<equiv> case p of (f1, f2, f3) \<Rightarrow> IImsupp11_1 (Rep_SSfun11 f1) \<union> IImsupp12_1 (Rep_SSfun12 f2) \<union> IImsupp21_1 (Rep_SSfun21 f3)"
-definition PFVars_2 :: "('var::{var_T1_pre,var_T2_pre}, 'tyvar::{var_T1_pre,var_T2_pre}, 'a::{var_T1_pre,var_T2_pre}, 'b) P \<Rightarrow> 'tyvar set" where
-  "PFVars_2 p \<equiv> case p of (f1, f2, f3) \<Rightarrow> IImsupp11_2 (Rep_SSfun11 f1) \<union> IImsupp12_2 (Rep_SSfun12 f2) \<union> IImsupp21_2 (Rep_SSfun21 f3)"
-
-definition Pmap :: "('var \<Rightarrow> 'var) \<Rightarrow> ('tyvar \<Rightarrow> 'tyvar) \<Rightarrow> ('var::{var_T1_pre,var_T2_pre}, 'tyvar::{var_T1_pre,var_T2_pre}, 'a::{var_T1_pre,var_T2_pre}, 'b) P \<Rightarrow> ('var, 'tyvar, 'a, 'b) P" where
-  "Pmap g1 g2 p \<equiv> case p of (f1, f2, f3) \<Rightarrow> (compSS11 g1 g2 f1, compSS12 g1 g2 f2, compSS21 g1 g2 f3)"
-
-definition avoiding_set1 :: "'var::{var_T1_pre,var_T2_pre} set" where "avoiding_set1 \<equiv> {}"
-definition avoiding_set2 :: "'tyvar::{var_T1_pre,var_T2_pre} set" where "avoiding_set2 \<equiv> {}"
-
-abbreviation "U1FVars_1 \<equiv> \<lambda>(_::('var, 'tyvar, 'a, 'b) T1) (x::('var::{var_T1_pre,var_T2_pre}, 'tyvar::{var_T1_pre,var_T2_pre}, 'a::{var_T1_pre,var_T2_pre}, 'b) T1). FFVars_T11 x"
-abbreviation "U1FVars_2 \<equiv> \<lambda>(_::('var, 'tyvar, 'a, 'b) T1) (x::('var::{var_T1_pre,var_T2_pre}, 'tyvar::{var_T1_pre,var_T2_pre}, 'a::{var_T1_pre,var_T2_pre}, 'b) T1). FFVars_T12 x"
-abbreviation "U2FVars_1 \<equiv> \<lambda>(_::('var, 'tyvar, 'a, 'b) T2) (x::('var::{var_T1_pre,var_T2_pre}, 'tyvar::{var_T1_pre,var_T2_pre}, 'a::{var_T1_pre,var_T2_pre}, 'b) T2). FFVars_T21 x"
-abbreviation "U2FVars_2 \<equiv> \<lambda>(_::('var, 'tyvar, 'a, 'b) T2) (x::('var::{var_T1_pre,var_T2_pre}, 'tyvar::{var_T1_pre,var_T2_pre}, 'a::{var_T1_pre,var_T2_pre}, 'b) T2). FFVars_T22 x"
-
-abbreviation "U1map \<equiv> \<lambda>f1 f2 (_::('var, 'tyvar, 'a, 'b) T1) (x::('var::{var_T1_pre,var_T2_pre}, 'tyvar::{var_T1_pre,var_T2_pre}, 'a::{var_T1_pre,var_T2_pre}, 'b) T1). rrename_T1 f1 f2 x"
-abbreviation "U2map \<equiv> \<lambda>f1 f2 (_::('var, 'tyvar, 'a, 'b) T2) (x::('var::{var_T1_pre,var_T2_pre}, 'tyvar::{var_T1_pre,var_T2_pre}, 'a::{var_T1_pre,var_T2_pre}, 'b) T2). rrename_T2 f1 f2 x"
-
-(**********************************************************************)
-(*                               PROOFS                               *)
-(**********************************************************************)
-
-lemmas Cinfinite_UNIV = conjI[OF T1_pre.UNIV_cinfinite card_of_Card_order]
-lemmas Cinfinite_card = cmin_Cinfinite[OF Cinfinite_UNIV Cinfinite_UNIV]
-lemmas regularCard_card = cmin_regularCard[OF T1_pre.var_regular T1_pre.var_regular Cinfinite_UNIV Cinfinite_UNIV]
-lemmas Un_bound = regularCard_Un[OF conjunct2[OF Cinfinite_card] conjunct1[OF Cinfinite_card] regularCard_card]
-lemmas UNION_bound = regularCard_UNION[OF conjunct2[OF Cinfinite_card] conjunct1[OF Cinfinite_card] regularCard_card]
 
 lemma VVr_injs:
   "VVr11 x = VVr11 x' \<Longrightarrow> x = x'"
@@ -392,18 +382,6 @@ lemma compSS_comp0s:
     apply (unfold id_o o_id)?
     apply (rule ext)
     apply (rule trans[OF comp_apply])
-    apply (rule arg_cong[of _ _ Abs_SSfun11])
-    apply (unfold comp_assoc)
-    apply (rule arg_cong2[OF refl, of _ _ "(\<circ>)"])
-    apply (rule trans)
-     apply (rule arg_cong2[OF _ refl, of _ _ "(\<circ>)"])
-     apply (rule Abs_SSfun11_inverse)
-     apply (rule iffD2[OF mem_Collect_eq])
-     apply (rule SSupp_rename_bounds)
-         apply (rule g_prems)+
-     apply (rule SSupp_comp_bounds)
-      apply (rule iffD1[OF mem_Collect_eq Rep_SSfun11])
-     apply (rule supp_inv_bound g_prems)+
     apply (unfold comp_assoc)
     apply (rule refl)
     done
@@ -414,18 +392,6 @@ lemma compSS_comp0s:
     apply (unfold id_o o_id)?
     apply (rule ext)
     apply (rule trans[OF comp_apply])
-    apply (rule arg_cong[of _ _ Abs_SSfun12])
-    apply (unfold comp_assoc)
-    apply (rule arg_cong2[OF refl, of _ _ "(\<circ>)"])
-    apply (rule trans)
-     apply (rule arg_cong2[OF _ refl, of _ _ "(\<circ>)"])
-     apply (rule Abs_SSfun12_inverse)
-     apply (rule iffD2[OF mem_Collect_eq])
-     apply (rule SSupp_rename_bounds)
-         apply (rule g_prems)+
-     apply (rule SSupp_comp_bounds)
-      apply (rule iffD1[OF mem_Collect_eq Rep_SSfun12])
-     apply (rule supp_inv_bound g_prems)+
     apply (unfold comp_assoc)
     apply (rule refl)
     done
@@ -436,18 +402,6 @@ lemma compSS_comp0s:
     apply (unfold id_o o_id)?
     apply (rule ext)
     apply (rule trans[OF comp_apply])
-    apply (rule arg_cong[of _ _ Abs_SSfun21])
-    apply (unfold comp_assoc)
-    apply (rule arg_cong2[OF refl, of _ _ "(\<circ>)"])
-    apply (rule trans)
-     apply (rule arg_cong2[OF _ refl, of _ _ "(\<circ>)"])
-     apply (rule Abs_SSfun21_inverse)
-     apply (rule iffD2[OF mem_Collect_eq])
-     apply (rule SSupp_rename_bounds)
-         apply (rule g_prems)+
-     apply (rule SSupp_comp_bounds)
-      apply (rule iffD1[OF mem_Collect_eq Rep_SSfun21])
-     apply (rule supp_inv_bound g_prems)+
     apply (unfold comp_assoc)
     apply (rule refl)
     done
@@ -457,59 +411,9 @@ lemma compSS_id0s:
   "compSS11 id id = id"
   "compSS12 id id = id"
   "compSS21 id id = id"
-  apply (unfold compSS11_def compSS12_def compSS21_def T1.rrename_id0s id_o o_id inv_id Rep_SSfun11_inverse Rep_SSfun12_inverse Rep_SSfun21_inverse)
+  apply (unfold compSS11_def compSS12_def compSS21_def T1.rrename_id0s id_o o_id inv_id)
   apply (unfold id_def)
   apply (rule refl)+
-  done
-
-lemma compSS_rep_eq:
-  fixes f1::"'var::{var_T1_pre, var_T2_pre} \<Rightarrow> 'var" and f2::"'tyvar::{var_T1_pre, var_T2_pre} \<Rightarrow> 'tyvar"
-  assumes f_prems: "bij f1" "|supp f1| <o cmin |UNIV::'var set| |UNIV::'tyvar set|" "bij f2" "|supp f2| <o cmin |UNIV::'var set| |UNIV::'tyvar set|"
-  shows
-    "Rep_SSfun11 (compSS11 f1 f2 p) = rrename_T1 f1 f2 \<circ> Rep_SSfun11 p \<circ> inv f1"
-    "Rep_SSfun12 (compSS12 f1 f2 p2) = rrename_T1 f1 f2 \<circ> Rep_SSfun12 p2 \<circ> inv f2"
-    "Rep_SSfun21 (compSS21 f1 f2 p3) = rrename_T2 f1 f2 \<circ> Rep_SSfun21 p3 \<circ> inv f1"
-  subgoal
-    apply (unfold compSS11_def)
-    apply (rule trans)
-     apply (rule Abs_SSfun11_inverse)
-     apply (rule iffD2[OF mem_Collect_eq])
-     apply (unfold comp_assoc)[1]
-     apply (rule SSupp_rename_bounds)
-         apply (rule assms)+
-     apply (rule SSupp_comp_bounds)
-      apply (rule iffD1[OF mem_Collect_eq Rep_SSfun11])
-     apply (rule supp_inv_bound assms)+
-    apply (rule refl)
-    done
-      (* copied from above *)
-  subgoal
-    apply (unfold compSS12_def)
-    apply (rule trans)
-     apply (rule Abs_SSfun12_inverse)
-     apply (rule iffD2[OF mem_Collect_eq])
-     apply (unfold comp_assoc)[1]
-     apply (rule SSupp_rename_bounds)
-         apply (rule assms)+
-     apply (rule SSupp_comp_bounds)
-      apply (rule iffD1[OF mem_Collect_eq Rep_SSfun12])
-     apply (rule supp_inv_bound assms)+
-    apply (rule refl)
-    done
-      (* copied from above *)
-  subgoal
-    apply (unfold compSS21_def)
-    apply (rule trans)
-     apply (rule Abs_SSfun21_inverse)
-     apply (rule iffD2[OF mem_Collect_eq])
-     apply (unfold comp_assoc)[1]
-     apply (rule SSupp_rename_bounds)
-         apply (rule assms)+
-     apply (rule SSupp_comp_bounds)
-      apply (rule iffD1[OF mem_Collect_eq Rep_SSfun21])
-     apply (rule supp_inv_bound assms)+
-    apply (rule refl)
-    done
   done
 
 lemma Pmap_id0: "Pmap id id = id"
@@ -699,7 +603,7 @@ lemma PFVars_Pmaps:
     "PFVars_2 (Pmap f1 f2 p) = f2 ` PFVars_2 p"
   subgoal
     apply (unfold Pmap_def PFVars_1_def case_prod_beta fst_conv snd_conv)
-    apply (unfold compSS_rep_eq[OF assms] image_Un)
+    apply (unfold compSS_defs image_Un)
     apply (rule arg_cong2[of _ _ _ _ "(\<union>)"])+
       (* REPEAT_DETERM *)
       apply (unfold IImsupp11_1_def)
@@ -744,7 +648,7 @@ lemma PFVars_Pmaps:
     done
   subgoal
     apply (unfold Pmap_def PFVars_2_def case_prod_beta fst_conv snd_conv)
-    apply (unfold compSS_rep_eq[OF assms] image_Un)
+    apply (unfold compSS_defs image_Un)
     apply (rule arg_cong2[of _ _ _ _ "(\<union>)"])+
       (* REPEAT_DETERM *)
       apply (unfold IImsupp11_2_def)
@@ -1060,20 +964,15 @@ lemma IImsupp_rrename_commute:
 lemma compSS_cong_ids:
   fixes f1::"'var::{var_T1_pre, var_T2_pre} \<Rightarrow> 'var" and f2::"'tyvar::{var_T1_pre, var_T2_pre} \<Rightarrow> 'tyvar"
   assumes f_prems: "bij f1" "|supp f1| <o |UNIV::'var set|" "bij f2" "|supp f2| <o |UNIV::'tyvar set|"
-  shows "(\<And>a. a \<in> IImsupp11_1 (Rep_SSfun11 p) \<Longrightarrow> f1 a = a) \<Longrightarrow> (\<And>a. a \<in> IImsupp11_2 (Rep_SSfun11 p) \<Longrightarrow> f2 a = a) \<Longrightarrow>
-    compSS11 f1 f2 p = p"
-    "(\<And>a. a \<in> IImsupp12_1 (Rep_SSfun12 p2) \<Longrightarrow> f1 a = a) \<Longrightarrow> (\<And>a. a \<in> IImsupp12_2 (Rep_SSfun12 p2) \<Longrightarrow> f2 a = a) \<Longrightarrow>
-    compSS12 f1 f2 p2 = p2"
-    "(\<And>a. a \<in> IImsupp21_1 (Rep_SSfun21 p3) \<Longrightarrow> f1 a = a) \<Longrightarrow> (\<And>a. a \<in> IImsupp21_2 (Rep_SSfun21 p3) \<Longrightarrow> f2 a = a) \<Longrightarrow>
-    compSS21 f1 f2 p3 = p3"
+  shows "(\<And>a. a \<in> IImsupp11_1 h1 \<Longrightarrow> f1 a = a) \<Longrightarrow> (\<And>a. a \<in> IImsupp11_2 h1 \<Longrightarrow> f2 a = a) \<Longrightarrow>
+    compSS11 f1 f2 h1 = h1"
+    "(\<And>a. a \<in> IImsupp12_1 h2 \<Longrightarrow> f1 a = a) \<Longrightarrow> (\<And>a. a \<in> IImsupp12_2 h2 \<Longrightarrow> f2 a = a) \<Longrightarrow>
+    compSS12 f1 f2 h2 = h2"
+    "(\<And>a. a \<in> IImsupp21_1 h3 \<Longrightarrow> f1 a = a) \<Longrightarrow> (\<And>a. a \<in> IImsupp21_2 h3 \<Longrightarrow> f2 a = a) \<Longrightarrow>
+    compSS21 f1 f2 h3 = h3"
   subgoal
     apply (unfold compSS11_def)
-    apply (rule Abs_SSfun11_cases[of p])
-    apply hypsubst_thin
-    apply (rule arg_cong[of _ _ Abs_SSfun11])
-    apply (rule ext)
-    apply (unfold Abs_SSfun11_inverse)
-    subgoal premises prems for y x
+    subgoal premises prems
       apply (subst IImsupp_rrename_commute)
             apply (rule f_prems)+
         (* REPEAT_DETERM *)
@@ -1093,7 +992,6 @@ lemma compSS_cong_ids:
         apply (erule bij_not_eq_twice[rotated])
         apply (rule f_prems)
         (* copied from above *)
-
        apply (rule trans[OF Int_commute])
        apply (rule iffD2[OF disjoint_iff])
        apply (rule allI)
@@ -1120,12 +1018,7 @@ lemma compSS_cong_ids:
       (* copied from above *)
   subgoal
     apply (unfold compSS12_def)
-    apply (rule Abs_SSfun12_cases[of p2])
-    apply hypsubst_thin
-    apply (rule arg_cong[of _ _ Abs_SSfun12])
-    apply (rule ext)
-    apply (unfold Abs_SSfun12_inverse)
-    subgoal premises prems for y x
+    subgoal premises prems
       apply (subst IImsupp_rrename_commute)
             apply (rule f_prems)+
         (* REPEAT_DETERM *)
@@ -1172,12 +1065,7 @@ lemma compSS_cong_ids:
       (* copied from above *)
   subgoal
     apply (unfold compSS21_def)
-    apply (rule Abs_SSfun21_cases[of p3])
-    apply hypsubst_thin
-    apply (rule arg_cong[of _ _ Abs_SSfun21])
-    apply (rule ext)
-    apply (unfold Abs_SSfun21_inverse)
-    subgoal premises prems for y x
+    subgoal premises prems
       apply (subst IImsupp_rrename_commute)
             apply (rule f_prems)+
         (* REPEAT_DETERM *)
@@ -1236,24 +1124,18 @@ lemma Pmap_cong_id:
   done
 
 lemma small_PFVarss:
-  "|PFVars_1 (p::('var::{var_T1_pre,var_T2_pre}, 'tyvar::{var_T1_pre,var_T2_pre}, 'a::{var_T1_pre,var_T2_pre}, 'b) P)| <o cmin |UNIV::'var set| |UNIV::'tyvar set|"
-  "|PFVars_2 p| <o cmin |UNIV::'var set| |UNIV::'tyvar set|"
+  "valid_P p \<Longrightarrow> |PFVars_1 (p::('var::{var_T1_pre,var_T2_pre}, 'tyvar::{var_T1_pre,var_T2_pre}, 'a::{var_T1_pre,var_T2_pre}, 'b) P)| <o cmin |UNIV::'var set| |UNIV::'tyvar set|"
+  "valid_P p \<Longrightarrow> |PFVars_2 p| <o cmin |UNIV::'var set| |UNIV::'tyvar set|"
   subgoal
-    apply (unfold PFVars_1_def case_prod_beta IImsupp11_1_def IImsupp12_1_def IImsupp21_1_def comp_def)
-    apply (rule Un_bound UNION_bound
-        iffD1[OF mem_Collect_eq Rep_SSfun11] iffD1[OF mem_Collect_eq Rep_SSfun12] iffD1[OF mem_Collect_eq Rep_SSfun21]
-        T1.card_of_FFVars_bounds
-        cmin_greater card_of_Card_order
-        )+
+    apply (unfold PFVars_1_def case_prod_beta IImsupp11_1_def IImsupp12_1_def IImsupp21_1_def comp_def valid_P_def)
+    apply (erule conjE)+
+    apply (assumption | rule Un_bound UNION_bound T1.card_of_FFVars_bounds cmin_greater card_of_Card_order)+
     done
   (* copied from above *)
   subgoal
-    apply (unfold PFVars_2_def case_prod_beta IImsupp11_2_def IImsupp12_2_def IImsupp21_2_def comp_def)
-    apply (rule Un_bound UNION_bound
-        iffD1[OF mem_Collect_eq Rep_SSfun11] iffD1[OF mem_Collect_eq Rep_SSfun12] iffD1[OF mem_Collect_eq Rep_SSfun21]
-        T1.card_of_FFVars_bounds
-        cmin_greater card_of_Card_order
-        )+
+    apply (unfold PFVars_2_def case_prod_beta IImsupp11_2_def IImsupp12_2_def IImsupp21_2_def comp_def valid_P_def)
+    apply (erule conjE)+
+    apply (assumption | rule Un_bound UNION_bound T1.card_of_FFVars_bounds cmin_greater card_of_Card_order)+
     done
   done
 
@@ -1305,28 +1187,21 @@ lemma asVVr_VVrs:
     done
   done
 
-lemma U1FVars_subset_1: "set5_T1_pre (y::(_, _, 'a::{var_T1_pre,var_T2_pre}, 'b, _, _, _, _, _, _) T1_pre) \<inter> (PFVars_1 p \<union> avoiding_set1) = {} \<Longrightarrow>
-  (\<And>t pu p. (t, pu) \<in> set7_T1_pre y \<union> set8_T1_pre y \<Longrightarrow> U1FVars_1 t (pu p) \<subseteq> FFVars_T11 t \<union> PFVars_1 p \<union> avoiding_set1) \<Longrightarrow>
-  (\<And>t pu p. (t, pu) \<in> set9_T1_pre y \<union> set10_T1_pre y \<Longrightarrow> U2FVars_1 t (pu p) \<subseteq> FFVars_T21 t \<union> PFVars_1 p \<union> avoiding_set1) \<Longrightarrow>
+lemma U1FVars_subset_1: "valid_P p \<Longrightarrow> set5_T1_pre (y::(_, _, 'a::{var_T1_pre,var_T2_pre}, 'b, _, _, _, _, _, _) T1_pre) \<inter> (PFVars_1 p \<union> avoiding_set1) = {} \<Longrightarrow>
+  (\<And>t pu p. valid_P p \<Longrightarrow> (t, pu) \<in> set7_T1_pre y \<union> set8_T1_pre y \<Longrightarrow> U1FVars_1 t (pu p) \<subseteq> FFVars_T11 t \<union> PFVars_1 p \<union> avoiding_set1) \<Longrightarrow>
+  (\<And>t pu p. valid_P p \<Longrightarrow> (t, pu) \<in> set9_T1_pre y \<union> set10_T1_pre y \<Longrightarrow> U2FVars_1 t (pu p) \<subseteq> FFVars_T21 t \<union> PFVars_1 p \<union> avoiding_set1) \<Longrightarrow>
   U1FVars_1 (T1_ctor (map_T1_pre id id id id id id fst fst fst fst y)) (U1ctor y p) \<subseteq> FFVars_T11 (T1_ctor (map_T1_pre id id id id id id fst fst fst fst y)) \<union> PFVars_1 p \<union> avoiding_set1"
-  apply (unfold avoiding_set1_def Un_empty_right)
+  apply (unfold avoiding_set1_def Un_empty_right case_prod_beta)
   subgoal premises prems
-  apply (unfold U1ctor_def case_prod_beta)
-  apply (rule case_split)
-   apply (subst if_P)
-    apply assumption
+    apply (unfold U1ctor_def case_prod_beta)
+    apply (rule case_split)
+     apply (subst if_P)
+      apply assumption
      apply (unfold isVVr11_def)[1]
      apply (erule exE)
-     apply (rule iffD2[OF arg_cong2[of _ _ _ _ "(\<subseteq>)"]])
-       apply (rule arg_cong[of _ _ FFVars_T11])
-       apply (rule arg_cong2[OF refl, of _ _ "Rep_SSfun11"])
-       apply (rule trans)
-        apply (rule arg_cong[of _ _ asVVr11])
-        apply assumption
-       apply (rule asVVr_VVrs)
-    apply (rule arg_cong2[OF _ refl, of _ _ "(\<union>)"])
-      apply (rule arg_cong[of _ _ FFVars_T11])
-      apply assumption
+     apply (drule sym)
+     apply (erule subst)
+     apply (unfold asVVr_VVrs)
      apply (rule case_split[of "_ = _"])
       apply (rule iffD2[OF arg_cong2[OF _ refl, of _ _ "(\<subseteq>)"]])
        apply (rule arg_cong[of _ _ FFVars_T11])
@@ -1337,28 +1212,21 @@ lemma U1FVars_subset_1: "set5_T1_pre (y::(_, _, 'a::{var_T1_pre,var_T2_pre}, 'b,
      apply (rule UnI2)
      apply (unfold PFVars_1_def case_prod_beta IImsupp11_1_def SSupp11_def)[1]
      apply (tactic \<open>resolve_tac @{context} [BNF_Util.mk_UnIN 3 1] 1\<close>)
-     apply (rule UnI2)
+     apply (rule UnI2)?
      apply (rule UN_I)
       apply (rule iffD2[OF mem_Collect_eq])
       apply assumption
      apply (rule iffD2[OF arg_cong2[OF refl comp_apply, of "(\<in>)"]])
-    apply assumption
+     apply assumption
   apply (unfold if_not_P)
   apply (rule case_split)
    apply (subst if_P)
       apply assumption
-apply (unfold isVVr12_def)[1]
+     apply (unfold isVVr12_def)[1]
      apply (erule exE)
-     apply (rule iffD2[OF arg_cong2[of _ _ _ _ "(\<subseteq>)"]])
-       apply (rule arg_cong[of _ _ FFVars_T11])
-       apply (rule arg_cong2[OF refl, of _ _ "Rep_SSfun12"])
-       apply (rule trans)
-        apply (rule arg_cong[of _ _ asVVr12])
-        apply assumption
-       apply (rule asVVr_VVrs)
-    apply (rule arg_cong2[OF _ refl, of _ _ "(\<union>)"])
-      apply (rule arg_cong[of _ _ FFVars_T11])
-      apply assumption
+     apply (drule sym)
+     apply (erule subst)
+     apply (unfold asVVr_VVrs)
      apply (rule case_split[of "_ = _"])
       apply (rule iffD2[OF arg_cong2[OF _ refl, of _ _ "(\<subseteq>)"]])
        apply (rule arg_cong[of _ _ FFVars_T11])
@@ -1369,11 +1237,12 @@ apply (unfold isVVr12_def)[1]
      apply (rule UnI2)
      apply (unfold PFVars_1_def case_prod_beta IImsupp12_1_def SSupp12_def)[1]
      apply (tactic \<open>resolve_tac @{context} [BNF_Util.mk_UnIN 3 2] 1\<close>)
+     apply (rule UnI2)?
      apply (rule UN_I)
       apply (rule iffD2[OF mem_Collect_eq])
       apply assumption
      apply (rule iffD2[OF arg_cong2[OF refl comp_apply, of "(\<in>)"]])
-    apply assumption
+     apply assumption
   apply (unfold if_not_P)
   apply (unfold T1.FFVars_cctors)
   apply (subst T1_pre.set_map, (rule supp_id_bound bij_id)+)+
@@ -1387,6 +1256,7 @@ apply (unfold isVVr12_def)[1]
      apply (rule UN_mono[OF subset_refl])
      apply (rule prems)
      apply (unfold prod.collapse)
+    apply (rule prems)
      apply (erule UnI1 UnI2)
     apply (rule iffD2[OF arg_cong2[OF refl, of _ _ "(\<subseteq>)"]])
      apply (rule Diff_Un_disjunct)
@@ -1398,7 +1268,8 @@ apply (unfold isVVr12_def)[1]
       apply (rule empty_subsetI)
      apply (rule UN_mono[OF subset_refl])
      apply (rule prems)
-    apply (unfold prod.collapse)
+       apply (unfold prod.collapse)
+       apply (rule prems)
     apply (erule UnI1 UnI2)
      apply (rule subset_If)
       apply (unfold UN_empty')[1]
@@ -1406,6 +1277,7 @@ apply (unfold isVVr12_def)[1]
      apply (rule UN_mono[OF subset_refl])
      apply (rule prems)
     apply (unfold prod.collapse)
+    apply (rule prems)
    apply (erule UnI1 UnI2)
     apply (rule iffD2[OF arg_cong2[OF refl, of _ _ "(\<subseteq>)"]])
      apply (rule Diff_Un_disjunct)
@@ -1418,32 +1290,26 @@ apply (unfold isVVr12_def)[1]
      apply (rule UN_mono[OF subset_refl])
      apply (rule prems)
     apply (unfold prod.collapse)
+    apply (rule prems)
   apply (erule UnI1 UnI2)
   done
   done
 
-lemma U1FVars_subset_2: "set6_T1_pre (y::(_, _, 'a::{var_T1_pre,var_T2_pre}, 'b, _, _, _, _, _, _) T1_pre) \<inter> (PFVars_2 p \<union> avoiding_set2) = {} \<Longrightarrow>
-  (\<And>t pu p. (t, pu) \<in> set7_T1_pre y \<union> set8_T1_pre y \<Longrightarrow> U1FVars_2 t (pu p) \<subseteq> FFVars_T12 t \<union> PFVars_2 p \<union> avoiding_set2) \<Longrightarrow>
-  (\<And>t pu p. (t, pu) \<in> set9_T1_pre y \<union> set10_T1_pre y \<Longrightarrow> U2FVars_2 t (pu p) \<subseteq> FFVars_T22 t \<union> PFVars_2 p \<union> avoiding_set2) \<Longrightarrow>
+lemma U1FVars_subset_2: "valid_P p \<Longrightarrow> set6_T1_pre (y::(_, _, 'a::{var_T1_pre,var_T2_pre}, 'b, _, _, _, _, _, _) T1_pre) \<inter> (PFVars_2 p \<union> avoiding_set2) = {} \<Longrightarrow>
+  (\<And>t pu p. valid_P p \<Longrightarrow> (t, pu) \<in> set7_T1_pre y \<union> set8_T1_pre y \<Longrightarrow> U1FVars_2 t (pu p) \<subseteq> FFVars_T12 t \<union> PFVars_2 p \<union> avoiding_set2) \<Longrightarrow>
+  (\<And>t pu p. valid_P p \<Longrightarrow> (t, pu) \<in> set9_T1_pre y \<union> set10_T1_pre y \<Longrightarrow> U2FVars_2 t (pu p) \<subseteq> FFVars_T22 t \<union> PFVars_2 p \<union> avoiding_set2) \<Longrightarrow>
   U1FVars_2 (T1_ctor (map_T1_pre id id id id id id fst fst fst fst y)) (U1ctor y p) \<subseteq> FFVars_T12 (T1_ctor (map_T1_pre id id id id id id fst fst fst fst y)) \<union> PFVars_2 p \<union> avoiding_set2"
   apply (unfold avoiding_set2_def Un_empty_right)
   subgoal premises prems
   apply (unfold U1ctor_def case_prod_beta)
   apply (rule case_split)
    apply (subst if_P)
-    apply assumption
+      apply assumption
      apply (unfold isVVr11_def)[1]
      apply (erule exE)
-     apply (rule iffD2[OF arg_cong2[of _ _ _ _ "(\<subseteq>)"]])
-       apply (rule arg_cong[of _ _ FFVars_T12])
-       apply (rule arg_cong2[OF refl, of _ _ "Rep_SSfun11"])
-       apply (rule trans)
-        apply (rule arg_cong[of _ _ asVVr11])
-        apply assumption
-       apply (rule asVVr_VVrs)
-    apply (rule arg_cong2[OF _ refl, of _ _ "(\<union>)"])
-      apply (rule arg_cong[of _ _ FFVars_T12])
-      apply assumption
+     apply (drule sym)
+     apply (erule subst)
+     apply (unfold asVVr_VVrs)
      apply (rule case_split[of "_ = _"])
       apply (rule iffD2[OF arg_cong2[OF _ refl, of _ _ "(\<subseteq>)"]])
        apply (rule arg_cong[of _ _ FFVars_T12])
@@ -1459,23 +1325,16 @@ lemma U1FVars_subset_2: "set6_T1_pre (y::(_, _, 'a::{var_T1_pre,var_T2_pre}, 'b,
       apply (rule iffD2[OF mem_Collect_eq])
       apply assumption
      apply (rule iffD2[OF arg_cong2[OF refl comp_apply, of "(\<in>)"]])
-    apply assumption
+     apply assumption
   apply (unfold if_not_P)
   apply (rule case_split)
    apply (subst if_P)
       apply assumption
-apply (unfold isVVr12_def)[1]
+     apply (unfold isVVr12_def)[1]
      apply (erule exE)
-     apply (rule iffD2[OF arg_cong2[of _ _ _ _ "(\<subseteq>)"]])
-       apply (rule arg_cong[of _ _ FFVars_T12])
-       apply (rule arg_cong2[OF refl, of _ _ "Rep_SSfun12"])
-       apply (rule trans)
-        apply (rule arg_cong[of _ _ asVVr12])
-        apply assumption
-       apply (rule asVVr_VVrs)
-    apply (rule arg_cong2[OF _ refl, of _ _ "(\<union>)"])
-      apply (rule arg_cong[of _ _ FFVars_T12])
-      apply assumption
+     apply (drule sym)
+     apply (erule subst)
+     apply (unfold asVVr_VVrs)
      apply (rule case_split[of "_ = _"])
       apply (rule iffD2[OF arg_cong2[OF _ refl, of _ _ "(\<subseteq>)"]])
        apply (rule arg_cong[of _ _ FFVars_T12])
@@ -1486,12 +1345,12 @@ apply (unfold isVVr12_def)[1]
      apply (rule UnI2)
      apply (unfold PFVars_2_def case_prod_beta IImsupp12_2_def SSupp12_def)[1]
      apply (tactic \<open>resolve_tac @{context} [BNF_Util.mk_UnIN 3 2] 1\<close>)
-    apply (rule UnI2)?
+     apply (rule UnI2)?
      apply (rule UN_I)
       apply (rule iffD2[OF mem_Collect_eq])
       apply assumption
      apply (rule iffD2[OF arg_cong2[OF refl comp_apply, of "(\<in>)"]])
-    apply assumption
+     apply assumption
   apply (unfold if_not_P)
   apply (unfold T1.FFVars_cctors)
   apply (subst T1_pre.set_map, (rule supp_id_bound bij_id)+)+
@@ -1505,6 +1364,7 @@ apply (unfold isVVr12_def)[1]
      apply (rule UN_mono[OF subset_refl])
      apply (rule prems)
      apply (unfold prod.collapse)
+        apply (rule prems)
      apply (erule UnI1 UnI2)
     apply (rule iffD2[OF arg_cong2[OF refl, of _ _ "(\<subseteq>)"]])
      apply (rule Diff_Un_disjunct)
@@ -1516,7 +1376,8 @@ apply (unfold isVVr12_def)[1]
       apply (rule empty_subsetI)
      apply (rule UN_mono[OF subset_refl])
      apply (rule prems)
-    apply (unfold prod.collapse)
+       apply (unfold prod.collapse)
+       apply (rule prems)
     apply (erule UnI1 UnI2)
      apply (rule subset_If)
       apply (unfold UN_empty')[1]
@@ -1524,39 +1385,34 @@ apply (unfold isVVr12_def)[1]
      apply (rule UN_mono[OF subset_refl])
      apply (rule prems)
     apply (unfold prod.collapse)
+    apply (rule prems)
      apply (erule UnI2 UnI1 | rule UnI1)+
     apply (rule subset_If)
      apply (unfold UN_empty')[1]
      apply (rule empty_subsetI)
     apply (rule UN_mono[OF subset_refl])
     apply (rule prems)
-    apply (unfold prod.collapse)
+     apply (unfold prod.collapse)
+     apply (rule prems)
     apply (erule UnI2 UnI1 | rule UnI1)+
   done
   done
 
-lemma U2FVars_subset_1: "set5_T2_pre (y::(_, _, 'a::{var_T1_pre,var_T2_pre}, 'b, _, _, _, _, _, _) T2_pre) \<inter> (PFVars_1 p \<union> avoiding_set1) = {} \<Longrightarrow>
-  (\<And>t pu p. (t, pu) \<in> set7_T2_pre y \<union> set8_T2_pre y \<Longrightarrow> U1FVars_1 t (pu p) \<subseteq> FFVars_T11 t \<union> PFVars_1 p \<union> avoiding_set1) \<Longrightarrow>
-  (\<And>t pu p. (t, pu) \<in> set9_T2_pre y \<union> set10_T2_pre y \<Longrightarrow> U2FVars_1 t (pu p) \<subseteq> FFVars_T21 t \<union> PFVars_1 p \<union> avoiding_set1) \<Longrightarrow>
+lemma U2FVars_subset_1: "valid_P p \<Longrightarrow> set5_T2_pre (y::(_, _, 'a::{var_T1_pre,var_T2_pre}, 'b, _, _, _, _, _, _) T2_pre) \<inter> (PFVars_1 p \<union> avoiding_set1) = {} \<Longrightarrow>
+  (\<And>t pu p. valid_P p \<Longrightarrow> (t, pu) \<in> set7_T2_pre y \<union> set8_T2_pre y \<Longrightarrow> U1FVars_1 t (pu p) \<subseteq> FFVars_T11 t \<union> PFVars_1 p \<union> avoiding_set1) \<Longrightarrow>
+  (\<And>t pu p. valid_P p \<Longrightarrow> (t, pu) \<in> set9_T2_pre y \<union> set10_T2_pre y \<Longrightarrow> U2FVars_1 t (pu p) \<subseteq> FFVars_T21 t \<union> PFVars_1 p \<union> avoiding_set1) \<Longrightarrow>
   U2FVars_1 (T2_ctor (map_T2_pre id id id id id id fst fst fst fst y)) (U2ctor y p) \<subseteq> FFVars_T21 (T2_ctor (map_T2_pre id id id id id id fst fst fst fst y)) \<union> PFVars_1 p \<union> avoiding_set1"
   apply (unfold avoiding_set1_def Un_empty_right)
   subgoal premises prems
   apply (unfold U2ctor_def case_prod_beta)
   apply (rule case_split)
    apply (subst if_P)
-    apply assumption
+      apply assumption
      apply (unfold isVVr21_def)[1]
      apply (erule exE)
-     apply (rule iffD2[OF arg_cong2[of _ _ _ _ "(\<subseteq>)"]])
-       apply (rule arg_cong[of _ _ FFVars_T21])
-       apply (rule arg_cong2[OF refl, of _ _ "Rep_SSfun21"])
-       apply (rule trans)
-        apply (rule arg_cong[of _ _ asVVr21])
-        apply assumption
-       apply (rule asVVr_VVrs)
-    apply (rule arg_cong2[OF _ refl, of _ _ "(\<union>)"])
-      apply (rule arg_cong[of _ _ FFVars_T21])
-      apply assumption
+     apply (drule sym)
+     apply (erule subst)
+     apply (unfold asVVr_VVrs)
      apply (rule case_split[of "_ = _"])
       apply (rule iffD2[OF arg_cong2[OF _ refl, of _ _ "(\<subseteq>)"]])
        apply (rule arg_cong[of _ _ FFVars_T21])
@@ -1567,12 +1423,12 @@ lemma U2FVars_subset_1: "set5_T2_pre (y::(_, _, 'a::{var_T1_pre,var_T2_pre}, 'b,
      apply (rule UnI2)
      apply (unfold PFVars_1_def case_prod_beta IImsupp21_1_def SSupp21_def)[1]
      apply (tactic \<open>resolve_tac @{context} [BNF_Util.mk_UnIN 3 3] 1\<close>)
-     apply (rule UnI2)
+     apply (rule UnI2)?
      apply (rule UN_I)
       apply (rule iffD2[OF mem_Collect_eq])
       apply assumption
      apply (rule iffD2[OF arg_cong2[OF refl comp_apply, of "(\<in>)"]])
-    apply assumption
+     apply assumption
   apply (unfold if_not_P)
   apply (unfold T1.FFVars_cctors)
   apply (subst T2_pre.set_map, (rule supp_id_bound bij_id)+)+
@@ -1585,7 +1441,8 @@ lemma U2FVars_subset_1: "set5_T2_pre (y::(_, _, 'a::{var_T1_pre,var_T2_pre}, 'b,
       apply (rule empty_subsetI)
      apply (rule UN_mono[OF subset_refl])
      apply (rule prems)
-     apply (unfold prod.collapse)
+        apply (unfold prod.collapse)
+        apply (rule prems)
      apply (erule UnI1 UnI2)
     apply (rule iffD2[OF arg_cong2[OF refl, of _ _ "(\<subseteq>)"]])
      apply (rule Diff_Un_disjunct)
@@ -1597,7 +1454,8 @@ lemma U2FVars_subset_1: "set5_T2_pre (y::(_, _, 'a::{var_T1_pre,var_T2_pre}, 'b,
       apply (rule empty_subsetI)
      apply (rule UN_mono[OF subset_refl])
      apply (rule prems)
-    apply (unfold prod.collapse)
+       apply (unfold prod.collapse)
+       apply (rule prems)
     apply (erule UnI1 UnI2)
      apply (rule subset_If)
       apply (unfold UN_empty')[1]
@@ -1605,6 +1463,7 @@ lemma U2FVars_subset_1: "set5_T2_pre (y::(_, _, 'a::{var_T1_pre,var_T2_pre}, 'b,
      apply (rule UN_mono[OF subset_refl])
      apply (rule prems)
     apply (unfold prod.collapse)
+      apply (rule prems)
    apply (erule UnI1 UnI2)
     apply (rule iffD2[OF arg_cong2[OF refl, of _ _ "(\<subseteq>)"]])
      apply (rule Diff_Un_disjunct)
@@ -1617,32 +1476,26 @@ lemma U2FVars_subset_1: "set5_T2_pre (y::(_, _, 'a::{var_T1_pre,var_T2_pre}, 'b,
      apply (rule UN_mono[OF subset_refl])
      apply (rule prems)
     apply (unfold prod.collapse)
+     apply (rule prems)
   apply (erule UnI1 UnI2)
   done
   done
 
-lemma U2FVars_subset_2: "set6_T2_pre (y::('var::{var_T1_pre,var_T2_pre}, 'tyvar::{var_T1_pre,var_T2_pre}, 'a::{var_T1_pre,var_T2_pre}, 'b, _, _, _, _, _, _) T2_pre) \<inter> (PFVars_2 p \<union> avoiding_set2) = {} \<Longrightarrow>
-  (\<And>t pu p. (t, pu) \<in> set7_T2_pre y \<union> set8_T2_pre y \<Longrightarrow> U1FVars_2 t (pu p) \<subseteq> FFVars_T12 t \<union> PFVars_2 p \<union> avoiding_set2) \<Longrightarrow>
-  (\<And>t pu p. (t, pu) \<in> set9_T2_pre y \<union> set10_T2_pre y \<Longrightarrow> U2FVars_2 t (pu p) \<subseteq> FFVars_T22 t \<union> PFVars_2 p \<union> avoiding_set2) \<Longrightarrow>
+lemma U2FVars_subset_2: "valid_P p \<Longrightarrow> set6_T2_pre (y::('var::{var_T1_pre,var_T2_pre}, 'tyvar::{var_T1_pre,var_T2_pre}, 'a::{var_T1_pre,var_T2_pre}, 'b, _, _, _, _, _, _) T2_pre) \<inter> (PFVars_2 p \<union> avoiding_set2) = {} \<Longrightarrow>
+  (\<And>t pu p. valid_P p \<Longrightarrow> (t, pu) \<in> set7_T2_pre y \<union> set8_T2_pre y \<Longrightarrow> U1FVars_2 t (pu p) \<subseteq> FFVars_T12 t \<union> PFVars_2 p \<union> avoiding_set2) \<Longrightarrow>
+  (\<And>t pu p. valid_P p \<Longrightarrow> (t, pu) \<in> set9_T2_pre y \<union> set10_T2_pre y \<Longrightarrow> U2FVars_2 t (pu p) \<subseteq> FFVars_T22 t \<union> PFVars_2 p \<union> avoiding_set2) \<Longrightarrow>
   U2FVars_2 (T2_ctor (map_T2_pre id id id id id id fst fst fst fst y)) (U2ctor y p) \<subseteq> FFVars_T22 (T2_ctor (map_T2_pre id id id id id id fst fst fst fst y)) \<union> PFVars_2 p \<union> avoiding_set2"
   apply (unfold avoiding_set2_def Un_empty_right)
   subgoal premises prems
   apply (unfold U2ctor_def case_prod_beta)
   apply (rule case_split)
    apply (subst if_P)
-    apply assumption
+      apply assumption
      apply (unfold isVVr21_def)[1]
      apply (erule exE)
-     apply (rule iffD2[OF arg_cong2[of _ _ _ _ "(\<subseteq>)"]])
-       apply (rule arg_cong[of _ _ FFVars_T22])
-       apply (rule arg_cong2[OF refl, of _ _ "Rep_SSfun21"])
-       apply (rule trans)
-        apply (rule arg_cong[of _ _ asVVr21])
-        apply assumption
-       apply (rule asVVr_VVrs)
-    apply (rule arg_cong2[OF _ refl, of _ _ "(\<union>)"])
-      apply (rule arg_cong[of _ _ FFVars_T22])
-      apply assumption
+     apply (drule sym)
+     apply (erule subst)
+     apply (unfold asVVr_VVrs)
      apply (rule case_split[of "_ = _"])
       apply (rule iffD2[OF arg_cong2[OF _ refl, of _ _ "(\<subseteq>)"]])
        apply (rule arg_cong[of _ _ FFVars_T22])
@@ -1658,7 +1511,7 @@ lemma U2FVars_subset_2: "set6_T2_pre (y::('var::{var_T1_pre,var_T2_pre}, 'tyvar:
       apply (rule iffD2[OF mem_Collect_eq])
       apply assumption
      apply (rule iffD2[OF arg_cong2[OF refl comp_apply, of "(\<in>)"]])
-    apply assumption
+     apply assumption
   apply (unfold if_not_P)
   apply (unfold T1.FFVars_cctors)
   apply (subst T2_pre.set_map, (rule supp_id_bound bij_id)+)+
@@ -1671,7 +1524,8 @@ lemma U2FVars_subset_2: "set6_T2_pre (y::('var::{var_T1_pre,var_T2_pre}, 'tyvar:
       apply (rule empty_subsetI)
      apply (rule UN_mono[OF subset_refl])
      apply (rule prems)
-     apply (unfold prod.collapse)
+        apply (unfold prod.collapse)
+        apply (rule prems)
      apply (erule UnI1 UnI2)
     apply (rule iffD2[OF arg_cong2[OF refl, of _ _ "(\<subseteq>)"]])
      apply (rule Diff_Un_disjunct)
@@ -1684,6 +1538,7 @@ lemma U2FVars_subset_2: "set6_T2_pre (y::('var::{var_T1_pre,var_T2_pre}, 'tyvar:
      apply (rule UN_mono[OF subset_refl])
      apply (rule prems)
     apply (unfold prod.collapse)
+       apply (rule prems)
     apply (erule UnI1 UnI2)
      apply (rule subset_If)
       apply (unfold UN_empty')[1]
@@ -1691,13 +1546,15 @@ lemma U2FVars_subset_2: "set6_T2_pre (y::('var::{var_T1_pre,var_T2_pre}, 'tyvar:
      apply (rule UN_mono[OF subset_refl])
      apply (rule prems)
     apply (unfold prod.collapse)
+    apply (rule prems)
      apply (erule UnI1 UnI2)
     apply (rule subset_If)
      apply (unfold UN_empty')[1]
      apply (rule empty_subsetI)
     apply (rule UN_mono[OF subset_refl])
     apply (rule prems)
-    apply (unfold prod.collapse)
+     apply (unfold prod.collapse)
+     apply (rule prems)
     apply (erule UnI2 UnI1 | rule UnI1)+
   done
   done
@@ -1770,13 +1627,22 @@ fixes f1::"'var::{var_T1_pre, var_T2_pre} \<Rightarrow> 'var" and f2::"'tyvar::{
   apply (rule refl)
   done
 
-lemma U1map_Uctor: "bij f1 \<Longrightarrow> |supp (f1::'var::{var_T1_pre,var_T2_pre} \<Rightarrow> 'var)| <o cmin |UNIV::'var set| |UNIV::'tyvar set| \<Longrightarrow> bij f2 \<Longrightarrow> |supp (f2::'tyvar::{var_T1_pre,var_T2_pre} \<Rightarrow> 'tyvar)| <o cmin |UNIV::'var set| |UNIV::'tyvar set| \<Longrightarrow>
+lemma valid_Pmap: "valid_P p \<Longrightarrow>
+  bij f1 \<Longrightarrow> |supp (f1::'var::{var_T1_pre,var_T2_pre} \<Rightarrow> 'var)| <o cmin |UNIV::'var set| |UNIV::'tyvar set| \<Longrightarrow>
+  bij f2 \<Longrightarrow> |supp (f2::'tyvar::{var_T1_pre,var_T2_pre} \<Rightarrow> 'tyvar)| <o cmin |UNIV::'var set| |UNIV::'tyvar set| \<Longrightarrow>
+  valid_P (Pmap f1 f2 p)"
+  apply (unfold valid_P_def Pmap_def case_prod_beta compSS_defs fst_conv snd_conv)
+  apply (erule conjE)+
+  apply (assumption | rule conjI SSupp_comp_bounds SSupp_rename_bounds supp_inv_bound)+
+  done
+
+lemma U1map_Uctor: "valid_P p \<Longrightarrow> bij f1 \<Longrightarrow> |supp (f1::'var::{var_T1_pre,var_T2_pre} \<Rightarrow> 'var)| <o cmin |UNIV::'var set| |UNIV::'tyvar set| \<Longrightarrow> bij f2 \<Longrightarrow> |supp (f2::'tyvar::{var_T1_pre,var_T2_pre} \<Rightarrow> 'tyvar)| <o cmin |UNIV::'var set| |UNIV::'tyvar set| \<Longrightarrow>
   U1map f1 f2 (T1_ctor (map_T1_pre id id id id id id fst fst fst fst y)) (U1ctor y p)
 = U1ctor (map_T1_pre f1 f2 id id f1 f2
-    (\<lambda>(t, pu). (rrename_T1 f1 f2 t, \<lambda>p. U1map f1 f2 t (pu (Pmap (inv f1) (inv f2) p))))
-    (\<lambda>(t, pu). (rrename_T1 f1 f2 t, \<lambda>p. U1map f1 f2 t (pu (Pmap (inv f1) (inv f2) p))))
-    (\<lambda>(t, pu). (rrename_T2 f1 f2 t, \<lambda>p. U2map f1 f2 t (pu (Pmap (inv f1) (inv f2) p))))
-    (\<lambda>(t, pu). (rrename_T2 f1 f2 t, \<lambda>p. U2map f1 f2 t (pu (Pmap (inv f1) (inv f2) p))))
+    (\<lambda>(t, pu). (rrename_T1 f1 f2 t, \<lambda>p. if valid_P p then U1map f1 f2 t (pu (Pmap (inv f1) (inv f2) p)) else undefined))
+    (\<lambda>(t, pu). (rrename_T1 f1 f2 t, \<lambda>p. if valid_P p then U1map f1 f2 t (pu (Pmap (inv f1) (inv f2) p)) else undefined))
+    (\<lambda>(t, pu). (rrename_T2 f1 f2 t, \<lambda>p. if valid_P p then U2map f1 f2 t (pu (Pmap (inv f1) (inv f2) p)) else undefined))
+    (\<lambda>(t, pu). (rrename_T2 f1 f2 t, \<lambda>p. if valid_P p then U2map f1 f2 t (pu (Pmap (inv f1) (inv f2) p)) else undefined))
  y) (Pmap f1 f2 p)"
   apply (unfold U1ctor_def)
   apply (subst T1_pre.map_comp, (assumption | rule supp_id_bound bij_id ordLess_ordLeq_trans cmin1 cmin2 card_of_Card_order)+)+
@@ -1790,29 +1656,12 @@ lemma U1map_Uctor: "bij f1 \<Longrightarrow> |supp (f1::'var::{var_T1_pre,var_T2
    apply (unfold if_P if_not_P)
    apply (unfold isVVr11_def)[1]
    apply (erule exE)
-   apply (rule trans)
-    apply (rule arg_cong[of _ _ "rrename_T1 f1 f2"])
-    apply (rule arg_cong2[OF refl, of _ _ "Rep_SSfun11"])
-    apply (rule trans)
-     apply (rule arg_cong[of _ _ asVVr11])
-     apply assumption
-    apply (rule asVVr_VVrs)
-   apply (unfold Pmap_def case_prod_beta fst_conv snd_conv)[1]
-   apply (rule sym)
-   apply (rule trans)
-    apply (rule arg_cong2[OF refl, of _ _ Rep_SSfun11])
-    apply (rule trans)
-     apply (rule arg_cong[of _ _ asVVr11])
-     apply (rule trans)
-      apply (rule arg_cong[of _ _ "rrename_T1 f1 f2"])
-      apply assumption
-     apply (rule rrename_VVrs)
-        apply (assumption | rule ordLess_ordLeq_trans cmin1 cmin2 card_of_Card_order)+
-    apply (rule asVVr_VVrs)
-   apply (rule trans)
-    apply (rule compSS_rep_eq[THEN fun_cong])
-       apply assumption+
-   apply (unfold comp_def)[1]
+   apply (drule sym)
+  apply (erule subst)
+   apply (unfold Pmap_def case_prod_beta fst_conv snd_conv asVVr_VVrs)[1]
+   apply (subst rrename_VVrs)
+       apply (assumption | rule ordLess_ordLeq_trans cmin1 cmin2 card_of_Card_order)+
+   apply (unfold asVVr_VVrs compSS_defs comp_def)[1]
    apply (subst inv_simp1)
     apply assumption
    apply (rule refl)
@@ -1823,29 +1672,12 @@ lemma U1map_Uctor: "bij f1 \<Longrightarrow> |supp (f1::'var::{var_T1_pre,var_T2
    apply (unfold if_P if_not_P)
    apply (unfold isVVr12_def)[1]
    apply (erule exE)
-   apply (rule trans)
-    apply (rule arg_cong[of _ _ "rrename_T1 f1 f2"])
-    apply (rule arg_cong2[OF refl, of _ _ "Rep_SSfun12"])
-    apply (rule trans)
-     apply (rule arg_cong[of _ _ asVVr12])
-     apply assumption
-    apply (rule asVVr_VVrs)
-   apply (unfold Pmap_def case_prod_beta fst_conv snd_conv)[1]
-   apply (rule sym)
-   apply (rule trans)
-    apply (rule arg_cong2[OF refl, of _ _ Rep_SSfun12])
-    apply (rule trans)
-     apply (rule arg_cong[of _ _ asVVr12])
-     apply (rule trans)
-      apply (rule arg_cong[of _ _ "rrename_T1 f1 f2"])
-      apply assumption
-     apply (rule rrename_VVrs)
-        apply (assumption | rule ordLess_ordLeq_trans cmin1 cmin2 card_of_Card_order)+
-    apply (rule asVVr_VVrs)
-   apply (rule trans)
-    apply (rule compSS_rep_eq[THEN fun_cong])
-       apply assumption+
-   apply (unfold comp_def)[1]
+   apply (drule sym)
+  apply (erule subst)
+   apply (unfold Pmap_def case_prod_beta fst_conv snd_conv asVVr_VVrs)[1]
+   apply (subst rrename_VVrs)
+       apply (assumption | rule ordLess_ordLeq_trans cmin1 cmin2 card_of_Card_order)+
+   apply (unfold asVVr_VVrs compSS_defs comp_def)[1]
    apply (subst inv_simp1)
     apply assumption
    apply (rule refl)
@@ -1859,16 +1691,18 @@ lemma U1map_Uctor: "bij f1 \<Longrightarrow> |supp (f1::'var::{var_T1_pre,var_T2
   apply (subst trans[OF comp_apply[symmetric] fun_cong[OF Pmap_comp0]], (assumption | rule supp_inv_bound bij_imp_bij_inv)+)+
   apply (subst inv_o_simp1, assumption)+
   apply (unfold trans[OF fun_cong[OF Pmap_id0] id_apply])
+  apply (subst valid_Pmap, assumption+)+
+  apply (unfold if_True)
   apply (rule refl)
   done
 
-lemma U2map_Uctor: "bij f1 \<Longrightarrow> |supp (f1::'var::{var_T1_pre,var_T2_pre} \<Rightarrow> 'var)| <o cmin |UNIV::'var set| |UNIV::'tyvar set| \<Longrightarrow> bij f2 \<Longrightarrow> |supp (f2::'tyvar::{var_T1_pre,var_T2_pre} \<Rightarrow> 'tyvar)| <o cmin |UNIV::'var set| |UNIV::'tyvar set| \<Longrightarrow>
+lemma U2map_Uctor: "valid_P p \<Longrightarrow> bij f1 \<Longrightarrow> |supp (f1::'var::{var_T1_pre,var_T2_pre} \<Rightarrow> 'var)| <o cmin |UNIV::'var set| |UNIV::'tyvar set| \<Longrightarrow> bij f2 \<Longrightarrow> |supp (f2::'tyvar::{var_T1_pre,var_T2_pre} \<Rightarrow> 'tyvar)| <o cmin |UNIV::'var set| |UNIV::'tyvar set| \<Longrightarrow>
   U2map f1 f2 (T2_ctor (map_T2_pre id id id id id id fst fst fst fst y)) (U2ctor y p)
 = U2ctor (map_T2_pre f1 f2 id id f1 f2
-    (\<lambda>(t, pu). (rrename_T1 f1 f2 t, \<lambda>p. U1map f1 f2 t (pu (Pmap (inv f1) (inv f2) p))))
-    (\<lambda>(t, pu). (rrename_T1 f1 f2 t, \<lambda>p. U1map f1 f2 t (pu (Pmap (inv f1) (inv f2) p))))
-    (\<lambda>(t, pu). (rrename_T2 f1 f2 t, \<lambda>p. U2map f1 f2 t (pu (Pmap (inv f1) (inv f2) p))))
-    (\<lambda>(t, pu). (rrename_T2 f1 f2 t, \<lambda>p. U2map f1 f2 t (pu (Pmap (inv f1) (inv f2) p))))
+    (\<lambda>(t, pu). (rrename_T1 f1 f2 t, \<lambda>p. if valid_P p then U1map f1 f2 t (pu (Pmap (inv f1) (inv f2) p)) else undefined))
+    (\<lambda>(t, pu). (rrename_T1 f1 f2 t, \<lambda>p. if valid_P p then U1map f1 f2 t (pu (Pmap (inv f1) (inv f2) p)) else undefined))
+    (\<lambda>(t, pu). (rrename_T2 f1 f2 t, \<lambda>p. if valid_P p then U2map f1 f2 t (pu (Pmap (inv f1) (inv f2) p)) else undefined))
+    (\<lambda>(t, pu). (rrename_T2 f1 f2 t, \<lambda>p. if valid_P p then U2map f1 f2 t (pu (Pmap (inv f1) (inv f2) p)) else undefined))
  y) (Pmap f1 f2 p)"
   apply (unfold U2ctor_def)
   apply (subst T2_pre.map_comp, (assumption | rule supp_id_bound bij_id ordLess_ordLeq_trans cmin1 cmin2 card_of_Card_order)+)+
@@ -1882,29 +1716,12 @@ lemma U2map_Uctor: "bij f1 \<Longrightarrow> |supp (f1::'var::{var_T1_pre,var_T2
    apply (unfold if_P if_not_P)
    apply (unfold isVVr21_def)[1]
    apply (erule exE)
-   apply (rule trans)
-    apply (rule arg_cong[of _ _ "rrename_T2 f1 f2"])
-    apply (rule arg_cong2[OF refl, of _ _ "Rep_SSfun21"])
-    apply (rule trans)
-     apply (rule arg_cong[of _ _ asVVr21])
-     apply assumption
-    apply (rule asVVr_VVrs)
-   apply (unfold Pmap_def case_prod_beta fst_conv snd_conv)[1]
-   apply (rule sym)
-   apply (rule trans)
-    apply (rule arg_cong2[OF refl, of _ _ Rep_SSfun21])
-    apply (rule trans)
-     apply (rule arg_cong[of _ _ asVVr21])
-     apply (rule trans)
-      apply (rule arg_cong[of _ _ "rrename_T2 f1 f2"])
-      apply assumption
-     apply (rule rrename_VVrs)
-        apply (assumption | rule ordLess_ordLeq_trans cmin1 cmin2 card_of_Card_order)+
-    apply (rule asVVr_VVrs)
-   apply (rule trans)
-    apply (rule compSS_rep_eq[THEN fun_cong])
-       apply assumption+
-   apply (unfold comp_def)[1]
+   apply (drule sym)
+  apply (erule subst)
+   apply (unfold Pmap_def case_prod_beta fst_conv snd_conv asVVr_VVrs)[1]
+   apply (subst rrename_VVrs)
+       apply (assumption | rule ordLess_ordLeq_trans cmin1 cmin2 card_of_Card_order)+
+   apply (unfold asVVr_VVrs compSS_defs comp_def)[1]
    apply (subst inv_simp1)
     apply assumption
    apply (rule refl)
@@ -1918,6 +1735,8 @@ lemma U2map_Uctor: "bij f1 \<Longrightarrow> |supp (f1::'var::{var_T1_pre,var_T2
   apply (subst trans[OF comp_apply[symmetric] fun_cong[OF Pmap_comp0]], (assumption | rule supp_inv_bound bij_imp_bij_inv)+)+
   apply (subst inv_o_simp1, assumption)+
   apply (unfold trans[OF fun_cong[OF Pmap_id0] id_apply])
+  apply (subst valid_Pmap, assumption+)+
+  apply (unfold if_True)
   apply (rule refl)
   done
 
@@ -1928,6 +1747,7 @@ thm Pmap_cong_id
 thm PFVars_Pmaps
 thm small_PFVarss
 thm small_avoiding_sets
+thm valid_Pmap
 
 (* model1 axioms *)
 thm U1map_Uctor
@@ -1952,7 +1772,10 @@ val parameters = {
     @{term "avoiding_set2 :: 'tyvar::{var_T1_pre,var_T2_pre} set"}
   ],
   min_bound = true,
-  validity = NONE : { pred: term, valid_Pmap: Proof.context -> tactic } option,
+  validity = SOME {
+    pred = @{term "valid_P :: ('var::{var_T1_pre, var_T2_pre}, 'tyvar::{var_T1_pre, var_T2_pre}, 'a::{var_T1_pre, var_T2_pre}, 'b) P \<Rightarrow> _"},
+    valid_Pmap = fn ctxt => HEADGOAL (resolve_tac ctxt @{thms valid_Pmap} THEN_ALL_NEW assume_tac ctxt)
+  },
   axioms = {
     Pmap_id0 = fn ctxt => EVERY1 [
       resolve_tac ctxt [trans],
@@ -1962,7 +1785,7 @@ val parameters = {
     Pmap_comp0 = fn ctxt => resolve_tac ctxt @{thms fun_cong[OF Pmap_comp0[symmetric]]} 1 THEN REPEAT_DETERM (assume_tac ctxt 1),
     Pmap_cong_id = fn ctxt => resolve_tac ctxt @{thms Pmap_cong_id} 1 THEN REPEAT_DETERM (assume_tac ctxt 1 ORELSE Goal.assume_rule_tac ctxt 1),
     PFVars_Pmaps = replicate nvars (fn ctxt => resolve_tac ctxt @{thms PFVars_Pmaps} 1 THEN REPEAT_DETERM (assume_tac ctxt 1)),
-    small_PFVarss = replicate nvars (fn ctxt => resolve_tac ctxt @{thms small_PFVarss} 1),
+    small_PFVarss = replicate nvars (fn ctxt => resolve_tac ctxt @{thms small_PFVarss} 1 THEN assume_tac ctxt 1),
     small_avoiding_sets = replicate nvars (fn ctxt => resolve_tac ctxt @{thms small_avoiding_sets} 1)
   }
 };
